almost finally done proving inv_bij

main.lean
@@ -1,79 +1,11 @@
 import tactic.finish
+import tactic.ext
+import tactic.binder_matching
 import biject
+import tactic.converter.binders
 
 universes u1 u2 u3
 
-
-def id_bij {α : Sort u1 } : bijective (id : α → α ) :=  
-  begin
-   apply and.intro,
-        intros x1 x2,
-        simp,
-        intro y,
-      apply exists.intro,
-      rewrite id 
-  end
-
-
-theorem bij_refl : reflexive in_bijection :=
-  begin
-    intro A,
-      apply exists.intro,
-      apply id_bij,
-  end
-
-
-theorem bij_trans : transitive in_bijection :=
-  begin
-    intros A B C,
-    intros F G,
-    cases F with f hf,
-    cases G with g hg,
-    apply exists.intro,
-    apply comp_of_bij_bij f g,
-    apply and.intro,
-    apply hf,
-    apply hg
-  end
-
-theorem single_exists_unique {α : Sort u1} {p : α → Prop} :
-  (∃! a : α, p a) ↔ nonempty (subsingleton {a : α // p a}) :=
-  begin
-    split,
-      intro hyp,
-        apply nonempty.intro,
-        apply subsingleton.intro,
-        intro u,
-        intro b,
-        cases u,
-        cases b,
-        simp,
-        apply unique_of_exists_unique hyp u_property b_property,
-      intro hyp,
-      
-
-  end
-
-
-noncomputable def inverse {α : Sort u1} {β : Sort u2} (f : α → β) (p : bijective f) : β → α :=
-  λ y : β, (((iff.elim_left (bijective_equiv f)) p) y ).some
-
-
-
-theorem inv_bij {α : Sort u1} {β : Sort u2} (f : α → β) (p : bijective f) : bijective (inverse f p) :=
-  begin
-    apply and.intro,
-      intros y1 y2,
-      rewrite inverse,
-      simp,
-      intro u,
-      
-
-      
-
-
-      
-  end 
 
 
 /-axiom inv_bij {α : Sort u1} {β : Sort u2} (f : α → β) (p : bijective f) : bijective (inverse f p)-/
@@ -103,13 +35,6 @@ def denombrable (α : Sort u1) : Prop :=
 def prod_func_left {A : Sort u1} {B : Sort u2}  (f : A → B) (C : Sort u3) : pprod A C → pprod B C :=
   λ x : pprod A C , pprod.mk (f (x.fst))  x.snd
 
-
-
-theorem map_eq {A : Sort u1} {B : Sort u2} (f : A → B) (x1 x2 : A) :  x1 = x2 → f x1 = f x2 :=
-  begin
-    intro a,
-    rewrite a 
-  end
 
 
 theorem tf_l {A : Sort u1} {B : Sort u2} {x3 x4 :pprod A  B} : x3 = x4 →  x3.1 = x4.1 ∧ x3.2 = x4.2 :=
