src/biject.lean
@@ -1,4 +1,5 @@
 import tactic.interactive
+import tactic.finish
 
 
 
@@ -8,7 +9,6 @@ constant α : Sort u1
 constant β : Sort u2
 constant γ : Sort u3
 constant f : α → β 
-
 
 def injective {α : Sort u1} {β : Sort u2} (f : α → β ) : Prop :=
       ∀ (x1 x2 : α ), f x1 = f x2 → x1 = x2 
@@ -36,7 +36,7 @@ lemma forall_exists_unique_imp_forall_exists {α : Sort u1} {β : Sort u2} {f : 
   end
 
 
-lemma fuck_this {α : Sort u1} {β : Sort u2} {f : α → β } {x1 x2 : α} : 
+lemma injective_of_bij_equiv {α : Sort u1} {β : Sort u2} {f : α → β } {x1 x2 : α} : 
   (∀ (y : β), ∃! (x : α), f x = y ) → f x1 = f x2 → x1 = x2 := 
   begin
     intro sup,
@@ -63,7 +63,7 @@ theorem bijective_equiv {α : Sort u1} {β : Sort u2} (f : α → β ) :
       intro sup,
         apply and.intro,
           intros x1 x2,
-          apply (fuck_this sup),
+          apply (injective_of_bij_equiv sup),
         intro a,
         apply (exists_of_exists_unique (sup a))
   end
@@ -107,3 +107,103 @@ theorem comp_of_bij_bij {α : Sort u1} {β : Sort u2} {γ  : Sort u3}  (f : α �
           apply and.elim_right (and.elim_left hyp),
           apply and.elim_right (and.elim_right hyp)
   end
+
+
+def id_bij {α : Sort u1 } : bijective (id : α → α ) :=  
+  begin
+   apply and.intro,
+        intros x1 x2,
+        simp,
+        intro y,
+      apply exists.intro,
+      rewrite id 
+  end
+
+
+theorem bij_refl : reflexive in_bijection :=
+  begin
+    intro A,
+      apply exists.intro,
+      apply id_bij,
+  end
+
+
+theorem bij_trans : transitive in_bijection :=
+  begin
+    intros A B C,
+    intros F G,
+    cases F with f hf,
+    cases G with g hg,
+    apply exists.intro,
+    apply comp_of_bij_bij f g,
+    apply and.intro,
+    apply hf,
+    apply hg
+  end
+
+
+lemma map_eq {A : Sort u1} {B : Sort u2} (f : A → B) {x1 x2 : A} :  x1 = x2 → f x1 = f x2 :=
+  begin
+    intro a,
+    rewrite a 
+  end
+
+
+
+theorem single_exists_unique {α : Type u1} {p : α → Prop} :
+  (∃! x : α, p x) ↔ nonempty {x : α // p x} ∧ subsingleton {x : α // p x} :=
+  begin
+    split,
+      intro hyp,
+      split,
+      use hyp.some,      
+      apply hyp.some_spec.left,
+      apply subsingleton.intro,
+      intros a b,
+      apply subtype.eq,
+      apply exists_unique.unique hyp a.property b.property,
+    intro hyp,
+    let sing := hyp.right,
+    apply exists_unique.intro,
+    let v : {x // p x} := (nonempty.some hyp.left),
+    exact v.property,
+    intro y,
+    intro h,
+    let u : {x // p x} := {val := y, property := h},
+    apply map_eq subtype.val  (@subsingleton.elim {x : α // p x} sing u (nonempty.some hyp.left))
+  end
+
+
+noncomputable def inverse {α : Sort u1} {β : Sort u2} (f : α → β) (p : bijective f) : β → α :=
+  λ y : β, (((iff.elim_left (bijective_equiv f)) p) y ).some
+
+constant p : bijective f
+constant x: α 
+
+
+lemma retard {α : Sort u1} {β : Sort u2} {f : α → β} {p : bijective f} {x : β} {y : α} :
+   (inverse f p x = y) = ((λ x : β,inverse f p x = y) x) :=
+  by simp
+
+theorem inv_bij {α : Sort u1} {β : Sort u2} (f : α → β) (p : bijective f) : bijective (inverse f p) :=
+  begin
+    apply iff.elim_right (bijective_equiv (inverse f p)),
+    intro y,
+    split,
+    split,
+      simp,
+      show (inverse f p (f y) = y),
+      rewrite inverse,
+      simp,
+      apply p.left (Exists.some _) (y) 
+        ((Exists.some_spec (inverse._proof_1 f p (f y))).left),
+    intro x,
+    simp,
+    rewrite inverse,
+    simp,
+    intro hyp,
+    sorry
+
+    
+        
+  end 
